EvmYul/EVM/PrecompiledContracts.lean
@@ -37,16 +37,52 @@ def Ξ_ECREC
     let r' : UInt256 := fromBytesBigEndian r.data.data
     let s' : UInt256 := fromBytesBigEndian s.data.data
     let o :=
-      match ECDSARECOVER h v r s with
-        | .ok s =>
-          if v' < 27 || 28 < v' || r' = 0 || r' >= secp256k1n || s' = 0 || s' >= secp256k1n then
-            .empty
-          else
-            ByteArray.zeroes ⟨12⟩ ++ (KEC s).extract 12 32
-        | .error e =>
-          dbg_trace s!"Ξ_ECREC failed: {e}"
-          .empty
+      if v' < 27 || 28 < v' || r' = 0 || r' >= secp256k1n || s' = 0 || s' >= secp256k1n then
+        .empty
+      else
+        -- dbg_trace h
+        -- dbg_trace v
+        -- dbg_trace r
+        -- dbg_trace s
+        match ECDSARECOVER h (BE (v' - 27)) r s with
+          | .ok s =>
+              ByteArray.zeroes ⟨12⟩ ++ (KEC s).extract 12 32
+          | .error e =>
+            dbg_trace s!"Ξ_ECREC failed: {e}"
+        .empty
     (σ, g - gᵣ, A, o)
+
+def longInput := "Lean 4 is a reimplementation of the Lean theorem prover in Lean itself. The new compiler produces C code, and users can now implement efficient proof automation in Lean, compile it into efficient C code, and load it as a plugin. In Lean 4, users can access all internal data structures used to implement Lean by merely importing the Lean package."
+
+-- Example taken from EllipticCurves.lean
+private def ecrecOutput :=
+  let (_, _, _, o) :=
+    Ξ_ECREC
+      default
+      3000
+      default
+      { (default : ExecutionEnv) with
+        inputData := h ++ v ++ r ++ s
+      }
+  o
+ where
+  h :=
+    UInt256.toByteArray 0x9a59efbc471b53491c8038fd5d5fe3be0a229873302bafba90c19fbe7d7c7f35
+  v :=
+    UInt256.toByteArray 0x1b
+  r :=
+    UInt256.toByteArray 0xd40b91381e1eeca34f4858a79ff4f3165066f93a76ba0f067848a962312f18ef
+  s :=
+    UInt256.toByteArray 0x0e86fce48de10c6b4e07b0a175877bc824bbf6d2089a50f3b11e24ad0d5c8173
+
+private example :
+  ecrecOutput
+    =
+  (ByteArray.ofBlob
+    "0000000000000000000000000bed7abd61247635c1973eb38474a2516ed1d884"
+  ).toOption
+:=
+  by native_decide
 
 def Ξ_SHA256
   (σ : AccountMap)
@@ -74,6 +110,22 @@ def Ξ_SHA256
           .empty
     (σ, g - gᵣ, A, o)
 
+private def shaOutput :=
+  let (_, _, _, o) :=
+    Ξ_SHA256
+      default
+      3000
+      default
+      { (default : ExecutionEnv) with
+        inputData := longInput.toUTF8
+      }
+  o
+private example :
+  EvmYul.toHex shaOutput
+    =
+  "4dbbf25c7844e6087e0a6948a71949c0ae2d46e75c16859457c430b8ce2d72ae"
+:= by native_decide
+
 def Ξ_RIP160
   (σ : AccountMap)
   (g : UInt256)
@@ -100,6 +152,22 @@ def Ξ_RIP160
           .empty
     (σ, g - gᵣ, A, o)
 
+private def ripOutput :=
+  let (_, _, _, o) :=
+    Ξ_RIP160
+      default
+      3000
+      default
+      { (default : ExecutionEnv) with
+        inputData := longInput.toUTF8
+      }
+  o
+
+private example :
+  EvmYul.toHex ripOutput = "5cff4c1668e5542c74a609a3146427c28e51ff5a"
+:= by native_decide
+
+
 def Ξ_ID
   (σ : AccountMap)
   (g : UInt256)
@@ -120,6 +188,21 @@ def Ξ_ID
   else
     let o := I.inputData
     (σ, g - gᵣ, A, o)
+
+private def idOutput :=
+  let (_, _, _, o) :=
+    Ξ_ID
+      default
+      3000
+      default
+      { (default : ExecutionEnv) with
+        inputData := longInput.toUTF8
+      }
+  o
+
+private example :
+  idOutput = longInput.toUTF8
+:= by native_decide
 
 def expModAux (m : ℕ) (a : ℕ) (c : ℕ) : ℕ → ℕ
   | 0 => a % m
@@ -175,6 +258,30 @@ def Ξ_EXPMOD
 
   (σ, g - gᵣ, A, o)
 
+private def expmodOutput :=
+  let (_, _, _, o) :=
+    Ξ_EXPMOD
+      default
+      3000
+      default
+      { (default : ExecutionEnv) with
+        inputData := l_B ++ l_E ++ l_M ++ B ++ E ++ M
+      }
+  o
+ where
+  l_B : ByteArray := UInt256.toByteArray 2
+  l_E : ByteArray := UInt256.toByteArray 1
+  l_M : ByteArray := UInt256.toByteArray 1
+  B : ByteArray := ⟨#[1, 0]⟩ -- 2^8
+  E : ByteArray := ⟨#[2]⟩
+  M : ByteArray := ⟨#[100]⟩
+
+private example :
+  expmodOutput
+    = ⟨#[65536 % 100]⟩ -- (2^8) ^ 2 % 10
+:=
+  by native_decide
+
 def Ξ_BN_ADD
   (σ : AccountMap)
   (g : UInt256)
@@ -193,6 +300,44 @@ def Ξ_BN_ADD
     | .error e =>
       dbg_trace s!"Ξ_BN_ADD failed: {e}"
       (σ, g - gᵣ, A, .empty)
+
+private def bn_addOutput₀ :=
+  let (_, _, _, o) :=
+    Ξ_BN_ADD
+      default
+      3000
+      default
+      { (default : ExecutionEnv) with
+        inputData := x₁ ++ y₁ ++ x₂ ++ y₂
+      }
+  o
+ where
+  x₁ : ByteArray := UInt256.toByteArray 0
+  y₁ : ByteArray := UInt256.toByteArray 0
+  x₂ : ByteArray := UInt256.toByteArray 1
+  y₂ : ByteArray := UInt256.toByteArray 2
+
+private def bn_addOutput₁ :=
+  let (_, _, _, o) :=
+    Ξ_BN_ADD
+      default
+      3000
+      default
+      { (default : ExecutionEnv) with
+        inputData := bn_addOutput₀ ++ x ++ y
+      }
+  o
+ where
+  x : ByteArray := UInt256.toByteArray 1
+  y : ByteArray := UInt256.toByteArray 2
+
+-- #eval bn_addOutput == UInt256.toByteArray 1 ++ UInt256.toByteArray 2
+
+-- private example :
+--   expmodOutput
+--     = UInt256.toByteArray 21888242871839275222246405745257275088696311157297823662689037894645226208580 ++ UInt256.toByteArray 2
+-- :=
+--   by native_decide
 
 def Ξ_BN_MUL
   (σ : AccountMap)
@@ -213,6 +358,24 @@ def Ξ_BN_MUL
       dbg_trace s!"Ξ_BN_MUL failed: {e}"
       (σ, g - gᵣ, A, .empty)
 
+private def bn_mulOutput :=
+  let (_, _, _, o) :=
+    Ξ_BN_MUL
+      default
+      3000
+      default
+      { (default : ExecutionEnv) with
+        inputData := x₁ ++ y₁ ++ n
+      }
+  o
+ where
+  x₁ : ByteArray := UInt256.toByteArray 1
+  y₁ : ByteArray := UInt256.toByteArray 2
+  n : ByteArray := UInt256.toByteArray 2
+
+-- (0, 0) + (1, 2) + (1, 2) = 2 * (1, 2)
+private example : bn_addOutput₁ = bn_mulOutput := by native_decide
+
 def Ξ_SNARKV
   (σ : AccountMap)
   (g : UInt256)
@@ -232,6 +395,24 @@ def Ξ_SNARKV
       dbg_trace s!"Ξ_SNARKV failed: {e}"
       (∅, 0, A, .empty)
 
+private def snarkvOutput :=
+  let (_, _, _, o) :=
+    Ξ_SNARKV
+      default
+      3000
+      default
+      { (default : ExecutionEnv) with
+        inputData := x ++ y ++ ByteArray.zeroes ⟨32 * 4⟩
+      }
+  o
+ where
+  x : ByteArray := UInt256.toByteArray 1
+  y : ByteArray := UInt256.toByteArray 2
+
+private example :
+  snarkvOutput.size = 32 ∧ (fromBytesBigEndian snarkvOutput.data.data) ∈ [0, 1]
+:= by native_decide
+
 def Ξ_BLAKE2_F
   (σ : AccountMap)
   (g : UInt256)
@@ -250,3 +431,26 @@ def Ξ_BLAKE2_F
     | .error e =>
       dbg_trace s!"Ξ_BLAKE2_F failed: {e}"
       (∅, 0, A, .empty)
+
+def blake2_fInput :=
+  ByteArray.ofBlob "0000000048c9bdf267e6096a3ba7ca8485ae67bb2bf894fe72f36e3cf1361d5f3af54fa5d182e6ad7f520e511f6c3e2b8c68059b6bbd41fbabd9831f79217e1319cde05b61626300000000000000000000000000000000000000000000000000000000000000000000000000000000000000000000000000000000000000000000000000000000000000000000000000000000000000000000000000000000000000000000000000000000000000000000000000000000000000000000000000000000000300000000000000000000000000000001"
+  |>.toOption.getD .empty
+
+private def blake2_fOutput :=
+  let (_, _, _, o) :=
+    Ξ_BLAKE2_F
+      default
+      3000
+      default
+      { (default : ExecutionEnv) with
+        inputData := blake2_fInput
+      }
+  o
+
+-- Example taken from
+-- https://eips.ethereum.org/EIPS/eip-152
+private example :
+  blake2_fOutput
+    =
+  (ByteArray.ofBlob "08c9bcf367e6096a3ba7ca8485ae67bb2bf894fe72f36e3cf1361d5f3af54fa5d282e6ad7f520e511f6c3e2b8c68059b9442be0454267ce079217e1319cde05b").toOption
+:= by native_decide
